feature: introduce the notion of value
Before this patch, the notion of memory location value was completely
absent. We introduce this notion within the Event type as a first
step towards true values handling.

src/Map/Map_def.v
@@ -1,44 +1,58 @@
-Require Import Coq.Structures.Equalities.
-Require Import Coq.Structures.DecidableType.
+Require Import SpecCert.Equality.
 
-Module Map (K:DecidableType).
-  Definition Kset := K.t.
+Definition Map
+           (K V: Type)
+          `{Eq K}
+  := K -> V.
 
-  Definition Map (t:Set) := Kset -> t.
-  (*Definition Map := fun (k:Kset) => init.*)
+Definition add_in_map
+           {K V: Type}
+          `{Eq K}
+           (m:   Map K V)
+           (k:   K)
+           (v:   V)
+  : Map K V :=
+  fun (k':K) => 
+    if eq_dec k k'
+    then v
+    else m k'.
 
-  Definition add_in_map {t:Set} (m:Map t) (k:Kset) (c:t):Map t :=
-    fun (k':Kset) => 
-      if K.eq_dec k k' then
-        c
-      else
-        m k'.
+Definition find_in_map
+           {K V: Type}
+          `{Eq K}
+           (m:   Map K V)
+           (k: K)
+  : V :=
+  m k.
 
-  Definition find_in_map {t:Set} (m:Map t) (k:Kset):t := m k.
+Lemma add_1
+      {K V: Type}
+     `{Eq K}
+      (m:   Map K V)
+      (k:   K)
+      (v:   V)
+  : find_in_map (add_in_map m k v) k = v.
+Proof.
+  unfold add_in_map.
+  unfold find_in_map.
+  destruct (eq_dec k k).
+  + reflexivity.
+  + destruct n.
+    apply (eq_refl k).
+Qed.
 
-  Lemma add_1: forall t:Set, forall m:Map t, forall k:Kset, forall c:t,
-          find_in_map (add_in_map m k c) k = c.
-  Proof.
-    intros t m k c.
-    unfold add_in_map.
-    unfold find_in_map.
-    destruct (K.eq_dec k k).
-    + reflexivity.
-    + unfold not in n.
-      assert (K.eq k k) by (apply K.eq_refl).
-      apply n in H.
-      destruct H.
-  Qed.
-
-  Lemma add_2: forall t:Set, forall m:Map t, forall k k', forall c:t,
-          ~ K.eq k k' -> find_in_map m k' = find_in_map (add_in_map m k c) k'.
-  Proof.
-    intros t m k k' c Hdiff.
-    unfold find_in_map, add_in_map.
-    destruct (K.eq_dec k k').
-    + unfold not in Hdiff.
-      apply Hdiff in e.
-      destruct e.
-    + reflexivity.
-  Qed.
-End Map.
+Lemma add_2
+      {K V:  Type}
+     `{Eq K}
+      (m:    Map K V)
+      (k k': K)
+      (v:    V)
+      (neq: ~ eq k k')
+  : find_in_map m k' = find_in_map (add_in_map m k v) k'.
+Proof.
+  unfold find_in_map, add_in_map.
+  destruct (eq_dec k k').
+  + apply neq in e.
+    destruct e.
+  + reflexivity.
+Qed.
