src/Address/AddressSpace.v
@@ -1,6 +1,5 @@
 Require Import SpecCert.Interval.
 
-Parameters (address_space:Interval)
-           (smram_space:Interval).
-
-Axiom (smram_is_in_space: is_included_in smram_space address_space).
+Parameters (address_space:     Interval)
+           (smram_space:       Interval)
+           (smram_is_in_space: is_included_in smram_space address_space).
