src/x86.v
@@ -1,4 +1,5 @@
 Require Export SpecCert.x86.Architecture.
 Require Export SpecCert.x86.Event.
+Require Export SpecCert.x86.Value.
 Require Export SpecCert.x86.Transition.
 Require Export SpecCert.x86.x86_def.
