src/Equality.v
@@ -1,0 +1,7 @@
+Class Eq
+      (T: Type)
+  := { eq: forall t t': T, Prop
+     ; eq_refl: forall t: T, eq t t
+     ; eq_sym: forall t t': T, eq t t' -> eq t' t
+     ; eq_trans: forall t t' t'': T, eq t t' -> eq t' t'' -> eq t t''
+     ; eq_dec: forall t t': T, {eq t t'} + {~ eq t t'} }.
